Creating files to store lemmas about state invariants. Progressing on proof of sitpn_to_hvhdl_bind_init_marking (40%)

common/GlobalFacts.v
@@ -18,7 +18,7 @@ Section SigEq.
 
   Variable A : Type.
   Variable P : A -> Prop.
-  Variable Aeqdec : forall x y : A, {x = y} + {x <> y}.
+  Variable eqA_dec : forall x y : A, {x = y} + {x <> y}.
   
   (** Two sigs are seq-equivalent if there first element is Leibniz's equal. *)
   
@@ -42,7 +42,7 @@ Section SigEq.
   (** Given that the equality is decidable for Set A, seq A is decidable. *)
   
   Definition seqdec (u v : {a : A | P a}) : {seq u v} + {~seq u v} :=
-    Aeqdec (proj1_sig u) (proj1_sig v).
+    eqA_dec (proj1_sig u) (proj1_sig v).
 
   (** Equivalence relation between two transitions that are elements of
     a subset of T. *)
@@ -56,20 +56,32 @@ Section SigEq.
     - right; inversion 1.
     - inversion IHlofA.
       + left; apply SetoidList.InA_cons; right; assumption.
-      + specialize (Aeqdec (proj1_sig a) (proj1_sig a0)) as Heqdec; inversion Heqdec;
+      + specialize (eqA_dec (proj1_sig a) (proj1_sig a0)) as Heqdec; inversion Heqdec;
           [ left; apply SetoidList.InA_cons; left; assumption |
             right; intro; inversion_clear H1; contradiction].
   Defined.
-
-  (** Declares seq as an instance of the Equivalence class. *)
-  
-  Instance Equivalence_seq : Equivalence seq :=
-    { Equivalence_Reflexive := seq_refl;
-      Equivalence_Symmetric := seq_sym;
-      Equivalence_Transitive := seq_trans }.
   
 End SigEq.
 
+(** Declares seq as an instance of the Equivalence class. *)
+  
+  Instance Equivalence_seq {A : Type} (P : A -> Prop) : Equivalence (@seq A P) :=
+    { Equivalence_Reflexive := (@seq_refl A P);
+      Equivalence_Symmetric := (@seq_sym A P);
+      Equivalence_Transitive := (@seq_trans A P) }.
+
+Add Parametric Relation {A : Type} {P : A -> Prop}
+    {eqA : A -> A -> Prop}
+    {eqA_dec : forall x y : A, {eqA x y} + {~eqA x y}} : ({ a : A | P a}) (@seq A P)
+    reflexivity proved by (@seq_refl A P)
+    symmetry proved by (@seq_sym A P)
+    transitivity proved by (@seq_trans A P)
+      as seq_rel.
+
 Arguments seq {A P}.
 Arguments seqdec {A P}.
+
+Hint Unfold seq : core.
+
+
 
