common/ListPlusFacts.v
@@ -1,7 +1,11 @@
 (** * More Facts about Lists *)
 
 Require Import common.Coqlib.
+Require Import common.InAndNoDup.
+Require Import common.FstSplit.
 Require Import common.ListPlus.
+Require Import common.SetoidListFacts.
+Require Import common.GlobalFacts.
 
 (** ** Facts about [Map] *)
 
@@ -46,4 +50,43 @@ Section FoldL.
   
 End FoldL.
 
+(** ** Facts about [Sig_in_List] *)
 
+Section SIL.
+
+  Lemma SIL_fs_setv :
+    forall {A B : Type} {P : A -> Prop}
+           {eqA_dec : forall x y : A, {x = y} + {x <> y}}
+           {x : {a | P a} } {v : B}
+           {l : list ({ a : A | P a} * B)},
+      Sig_in_List (fs l) -> Sig_in_List (fs (setv (seqdec eqA_dec) x v l)).
+  Proof.
+    intros until l; functional induction (setv (seqdec eqA_dec) x v l) using setv_ind.
+    (* CASE l = [] *)
+    intros SIL; destruct SIL as (InA_, NoDupA_); specialize (InA_ x).
+    inversion InA_.
+    (* CASE [eqk x a] *)
+    rewrite fs_eq_cons_app; intros SIL; cbn in SIL.
+    rewrite fs_eq_cons_app; cbn.
+    destruct SIL as (InA_, NoDupA_).
+    split.
+    intros y; specialize (InA_ y).
+    inversion_clear InA_;
+      [ eapply InA_cons_hd; unfold seq; rewrite _x; assumption | eauto ].
+    constructor; [  | eauto with setoidl ].
+    inversion_clear NoDupA_; clear e1; symmetry in _x; eauto 2 with setoidl typeclass_instances.    
+    (* CASE [~eqk x a] *)
+    rewrite fs_eq_cons_app; intros SIL; cbn in SIL.
+    rewrite fs_eq_cons_app; cbn.
+    destruct SIL as (InA_, NoDupA_).
+    split.
+    intros y; specialize (InA_ y).
+    inversion_clear InA_;
+      [ eapply InA_cons_hd; unfold seq; rewrite H; reflexivity | eauto with setoidl ].
+    eapply InA_cons_tl; eauto with setoidl.
+    eapply InA_fs_InA_fs_setv; eauto with typeclass_instances.
+    constructor; inversion NoDupA_; eauto 2 with setoidl typeclass_instances.
+  Qed.
+
+  
+End SIL.
