sitpn2hvhdl/GenerateArchitectureInvs.v
@@ -1,0 +1,326 @@
+(** * Architecture Generation and State Invariants *)
+
+Require Import String.
+Require Import common.Coqlib.
+Require Import common.StateAndErrorMonad.
+Require Import common.StateAndErrorMonadTactics.
+Require Import common.ListPlus.
+Require Import common.ListMonad.
+Require Import common.ListMonadFacts.
+Require Import common.ListMonadTactics.
+Require Import common.SetoidListFacts.
+
+Require Import dp.Sitpn.
+Require Import dp.SitpnFacts.
+
+Require Import hvhdl.Place.
+Require Import hvhdl.AbstractSyntax.
+
+Require Import sitpn2hvhdl.Sitpn2HVhdl.
+
+(** ** Place Map Generation and State Invariants *)
+
+Section GenPMapInvs.
+
+  Ltac solve_gen_pmap_entry_sinv :=
+    intros *; intros e; minv e;
+    match goal with
+    | [ H: _ ?st1 = OK _ _ |- ?f ?st1 = ?f ?st2 ] =>
+      solve_listm H;
+      match goal with
+      | [ H: _ ?st1 = OK _ ?st2,  H': _ = OK _ ?st3 |- _ ?st1 = _ ?st3 ] =>
+        transitivity (f st2);
+        [ solveSInv H; intros *; intros e; minv e; auto
+        | solveSInv H'; intros *; intros e; minv e; auto]
+      end
+    end.
+  
+  Lemma gen_pmap_entry_inv_γ :
+    forall {sitpn} {p : P sitpn} {mm s v s'},
+      generate_place_map_entry p mm s = OK v s' ->
+      γ s = γ s'.
+  Proof. try solve_gen_pmap_entry_sinv. Qed.
+
+  Lemma gen_pmap_inv_γ :
+    forall {sitpn mm s v s'},
+      @generate_place_map sitpn mm s = OK v s' ->
+      γ s = γ s'.
+  Proof.
+    intros until s'; intros e; minv e.
+    pattern s0, s3.
+    eapply map_inv_state; eauto with typeclass_instances; cbn.
+    intros; eapply gen_pmap_entry_inv_γ; eauto.
+  Qed.
+  
+  Lemma gen_pmap_entry_inv_lofPs :
+    forall {sitpn} {p : P sitpn} {mm s v s'},
+      generate_place_map_entry p mm s = OK v s' ->
+      lofPs s = lofPs s'.
+  Proof. try solve_gen_pmap_entry_sinv. Qed.
+
+  Lemma gen_pmap_inv_lofPs :
+    forall {sitpn mm s v s'},
+      @generate_place_map sitpn mm s = OK v s' ->
+      lofPs s = lofPs s'.
+  Proof.
+    intros until s'; intros e; minv e.
+    pattern s0, s3.
+    eapply map_inv_state; eauto with typeclass_instances; cbn.
+    intros; eapply gen_pmap_entry_inv_lofPs; eauto.
+  Qed.
+  
+End GenPMapInvs.
+
+(** ** Transition Map Generation and State Invariants *)
+
+Section GenTMapInvs.
+
+  Lemma gen_tmap_entry_inv_γ :
+    forall {sitpn} {t : T sitpn} {s v s'},
+      generate_trans_map_entry t s = OK v s' ->
+      γ s = γ s'.
+  Proof. intros until s'; intros e; minv e; solve_listm EQ1. Qed.
+
+  Lemma gen_tmap_inv_γ :
+    forall {sitpn s v s'},
+      @generate_trans_map sitpn s = OK v s' ->
+      γ s = γ s'.
+  Proof.
+    intros until s'; intros e; minv e.
+    pattern s0, s3.
+    eapply map_inv_state; eauto with typeclass_instances; cbn.
+    intros; eapply gen_tmap_entry_inv_γ; eauto.
+  Qed.
+  
+  Lemma gen_tmap_entry_inv_lofPs :
+    forall {sitpn} {t : T sitpn} {s v s'},
+      generate_trans_map_entry t s = OK v s' ->
+      lofPs s = lofPs s'.
+  Proof. intros until s'; intros e; minv e; solve_listm EQ1. Qed.
+
+  Lemma gen_tmap_inv_lofPs :
+    forall {sitpn s v s'},
+      @generate_trans_map sitpn s = OK v s' ->
+      lofPs s = lofPs s'.
+  Proof.
+    intros until s'; intros e; minv e.
+    pattern s0, s3.
+    eapply map_inv_state; eauto with typeclass_instances; cbn.
+    intros; eapply gen_tmap_entry_inv_lofPs; eauto.
+  Qed.
+  
+End GenTMapInvs.
+
+(** ** Interconnection Generation and State Invariants *)
+
+Section GenInterconnInvs.
+
+  Lemma connect_fired_port_inv_γ :
+    forall {sitpn} {e} {t : T sitpn} {s v s'},
+      connect_fired_port e t s = OK v s' ->
+      γ s = γ s'.
+  Proof.
+    intros *; intros e1; monadFullInv e1;
+      solve_listm EQ3; unfold get_actual_of_out_port in EQ1; destrm EQ1;
+        monadInv EQ1; destrm EQ2; inversion EQ2; auto.    
+  Qed.
+
+  Lemma connect_fired_port_inv_lofPs :
+    forall {sitpn} {e} {t : T sitpn} {s v s'},
+      connect_fired_port e t s = OK v s' ->
+      lofPs s = lofPs s'.
+  Proof. intros *; intros e1; minv e1; solve_listm EQ1. Qed.
+
+  Lemma connect_fired_port_inv_plmap :
+    forall {sitpn} {e} {t : T sitpn} {s v s'},
+      connect_fired_port e t s = OK v s' ->
+      plmap (arch s) = plmap (arch s').
+  Proof. intros *; intros e1; minv e1; solve_listm EQ1. Qed.
+      
+  Lemma connect_fired_ports_inv_γ :
+    forall {sitpn} {lofTs : list (T sitpn)} {s v s'},
+      connect_fired_ports lofTs s = OK v s' ->
+      γ s = γ s'.            
+  Proof. intros *; intros e; unfold connect_fired_ports in e; solve_listm e.
+         intros; eapply connect_fired_port_inv_γ; eauto.
+  Qed.
+
+  Lemma connect_fired_ports_inv_lofPs :
+    forall {sitpn} {lofTs : list (T sitpn)} {s v s'},
+      connect_fired_ports lofTs s = OK v s' ->
+      lofPs s = lofPs s'.            
+  Proof.
+    intros *; intros e; unfold connect_fired_ports in e; solve_listm e.
+    intros; eapply connect_fired_port_inv_lofPs; eauto.
+  Qed.
+
+  Lemma connect_fired_ports_inv_plmap :
+    forall {sitpn} {lofTs : list (T sitpn)} {s v s'},
+      connect_fired_ports lofTs s = OK v s' ->
+      plmap (arch s) = plmap (arch s').            
+  Proof.
+    intros *; intros e; unfold connect_fired_ports in e; solve_listm e.
+    intros; eapply connect_fired_port_inv_plmap; eauto.
+  Qed.
+  
+  Lemma connect_inv_γ :
+    forall {sitpn xcomp ycomp id__x id__y} {s : Sitpn2HVhdlState sitpn} {v s'},
+      connect xcomp ycomp id__x id__y s  = OK v s' ->
+      γ s = γ s'.
+  Proof. intros until s'; intros e; minv e; simpl; reflexivity. Qed.
+
+  Lemma connect_inv_lofPs :
+    forall {sitpn xcomp ycomp id__x id__y} {s : Sitpn2HVhdlState sitpn} {v s'},
+      connect xcomp ycomp id__x id__y s  = OK v s' ->
+      lofPs s = lofPs s'.
+  Proof. intros until s'; intros e; minv e; simpl; reflexivity. Qed.
+
+  Lemma connect_inv_plmap :
+    forall {sitpn xcomp ycomp id__x id__y} {s : Sitpn2HVhdlState sitpn} {v s'},
+      connect xcomp ycomp id__x id__y s  = OK v s' ->
+      plmap (arch s) = plmap (arch s').
+  Proof. intros until s'; intros e; minv e; simpl; reflexivity. Qed.
+  
+  Lemma connect_poutputs_inv_γ :
+    forall {sitpn} {pinfo : PlaceInfo sitpn} {hcomp s v s'},
+      connect_place_outputs pinfo hcomp s = OK v s' ->
+      γ s = γ s'.
+  Proof.
+    intros *; intros e; unfold connect_place_outputs in e; solve_listm e.
+    intros *; intros e; monadInv e; minv EQ; solve_listm EQ3. 
+    rewrite (connect_inv_γ EQ1); clear EQ1.
+    destrm EQ2; monadInv EQ2; rewrite (connect_inv_γ EQ); clear EQ.
+    destrm EQ0; monadInv EQ0; rewrite (connect_inv_γ EQ); clear EQ.
+    minv EQ1; auto.
+  Qed.
+
+  Lemma connect_poutputs_inv_lofPs :
+    forall {sitpn} {pinfo : PlaceInfo sitpn} {hcomp s v s'},
+      connect_place_outputs pinfo hcomp s = OK v s' ->
+      lofPs s = lofPs s'.
+  Proof.
+    intros *; intros e; unfold connect_place_outputs in e; solve_listm e.
+    intros *; intros e; monadInv e; minv EQ; solve_listm EQ3. 
+    rewrite (connect_inv_lofPs EQ1); clear EQ1.
+    destrm EQ2; monadInv EQ2; rewrite (connect_inv_lofPs EQ); clear EQ.
+    destrm EQ0; monadInv EQ0; rewrite (connect_inv_lofPs EQ); clear EQ.
+    minv EQ1; auto.
+  Qed.
+
+  Lemma connect_poutputs_inv_plmap :
+    forall {sitpn} {pinfo : PlaceInfo sitpn} {hcomp s v s'},
+      connect_place_outputs pinfo hcomp s = OK v s' ->
+      plmap (arch s) = plmap (arch s').
+  Proof.
+    intros *; intros e; unfold connect_place_outputs in e; solve_listm e.
+    intros *; intros e; monadInv e; minv EQ; solve_listm EQ3. 
+    rewrite (connect_inv_plmap EQ1); clear EQ1.
+    destrm EQ2; monadInv EQ2; rewrite (connect_inv_plmap EQ); clear EQ.
+    destrm EQ0; monadInv EQ0; rewrite (connect_inv_plmap EQ); clear EQ.
+    minv EQ1; auto.
+  Qed.
+  
+  Lemma interconnect_p_inv_γ :
+    forall {sitpn} {p : P sitpn} {s v s'},
+      interconnect_p p s = OK v s' ->
+      γ s = γ s'.
+  Proof.
+    intros until s'; intros e; minv e; simpl.
+    solve_listm EQ4; solve_listm EQ5.
+    transitivity (γ s3).
+    erewrite connect_fired_ports_inv_γ; eauto.
+    transitivity (γ s2).
+    erewrite connect_fired_ports_inv_γ; eauto.
+    erewrite connect_poutputs_inv_γ; eauto.  
+  Qed.
+
+  Lemma interconnect_p_inv_lofPs :
+    forall {sitpn} {p : P sitpn} {s v s'},
+      interconnect_p p s = OK v s' ->
+      lofPs s = lofPs s'.
+  Proof.
+    intros until s'; intros e; minv e; simpl.
+    solve_listm EQ4; solve_listm EQ5.
+    transitivity (lofPs s3).
+    erewrite connect_fired_ports_inv_lofPs; eauto.
+    transitivity (lofPs s2).
+    erewrite connect_fired_ports_inv_lofPs; eauto.
+    erewrite connect_poutputs_inv_lofPs; eauto.  
+  Qed.
+  
+  Lemma interconnect_p_inv_pcomp :
+    forall {sitpn p1 s v s'},
+      @interconnect_p sitpn p1 s = OK v s' ->
+      forall p2,
+      (exists g i o, InA Pkeq (p2, (g, i, o)) (plmap (arch s))) ->
+      (exists g i o, InA Pkeq (p2, (g, i, o)) (plmap (arch s'))).
+  Proof.
+    intros until s'; intros e p2; minv e.
+    destruct (Peqdec p1 p2) as [Peq_ | nPeq].
+    (* CASE [Peq p1 p2] *)
+    destruct x2 as ((g1, i1), o1).
+    exists g1, i1, o1; eauto with setoidl.
+    (* CASE [~Peq p1 p2] *)
+    destruct 1 as (g1, (i1, (o1, InA_plmap))).
+    exists g1, i1, o1.
+    eapply InA_setv_inv_1; eauto.
+    assert (e : plmap (arch s0) = plmap (arch s5)).
+    { rewrite (getv_inv_state EQ4).
+      rewrite (getv_inv_state EQ5).
+      rewrite (connect_fired_ports_inv_plmap EQ3).
+      rewrite (connect_fired_ports_inv_plmap EQ0).
+      rewrite (connect_poutputs_inv_plmap EQ2).
+      reflexivity.
+    }
+    rewrite <- e; auto.
+    intros Peq_; symmetry in Peq_; contradiction.
+  Qed.
+    
+End GenInterconnInvs.
+
+(** ** Facts about Architecture Generation Function *)
+
+Lemma gen_arch_inv_γ :
+  forall {sitpn mm s v s'},
+    @generate_architecture sitpn mm s = OK v s' ->
+    γ s = γ s'.
+Proof.
+  intros until s'; intros e; minv e.
+  shelf_state EQ1; shelf_state EQ3.
+  transitivity (γ s4).
+  solve_listm EQ; intros; eapply gen_pmap_entry_inv_γ; eauto.
+  change (γ s4) with (γ s); transitivity (γ s5).
+  solve_listm EQ1; intros; eapply gen_tmap_entry_inv_γ; eauto.
+  change (γ s5) with (γ s1).
+  solve_listm EQ3; intros; eapply interconnect_p_inv_γ; eauto.
+Qed.
+
+Lemma gen_arch_inv_lofPs :
+  forall {sitpn mm s v s'},
+    @generate_architecture sitpn mm s = OK v s' ->
+    lofPs s = lofPs s'.
+Proof.
+  intros until s'; intros e; monadFullInv e.
+  shelf_state EQ1; shelf_state EQ3.
+  transitivity (lofPs s4).
+  solve_listm EQ; intros; eapply gen_pmap_entry_inv_lofPs; eauto.
+  change (lofPs s4) with (lofPs s); transitivity (lofPs s5).
+  solve_listm EQ1; intros; eapply gen_tmap_entry_inv_lofPs; eauto.
+  change (lofPs s5) with (lofPs s1).
+  solve_listm EQ3; intros; eapply interconnect_p_inv_lofPs; eauto.
+Qed.
+
+Lemma gen_arch_sil_plmap : 
+  forall {sitpn mm s v s'},
+    @generate_architecture sitpn mm s = OK v s' ->
+    Sig_in_List (lofPs s) ->
+    (forall p, ~InA Peq p (fs (plmap (arch s)))) ->
+    NoDupA Peq (fs (plmap (arch s))) ->
+    Sig_in_List (fs (plmap (arch s'))).
+Admitted.
+
+Lemma gen_arch_inv_beh :
+  forall {sitpn mm s v s'},
+    @generate_architecture sitpn mm s = OK v s' ->
+    beh s = beh s'.
+Admitted.
