sitpn2hvhdl/GenerateHVhdlFacts.v
@@ -3,54 +3,24 @@
 Require Import String.
 Require Import common.Coqlib.
 Require Import common.GlobalFacts.
-Require Import common.FstSplit.
-Require Import common.InAndNoDup.
-Require Import common.ListDep.
 Require Import common.StateAndErrorMonad.
 Require Import common.StateAndErrorMonadTactics.
-Require Import common.ListMonad.
-Require Import common.ListMonadFacts.
-Require Import common.ListMonadTactics.
-Require Import common.SetoidListFacts.
-Require Import common.ListPlus.
+Require Import common.ListLib.
 
-Require Import sitpn.dp.Sitpn.
-Require Import sitpn.dp.SitpnFacts.
-Require Import sitpn.dp.SitpnWellDefined.
-Require Import sitpn.dp.SitpnWellDefinedTactics.
+Require Import sitpn.dp.SitpnLib.
 
 Require Import hvhdl.HVhdlTypes.
 Require Import hvhdl.AbstractSyntax.
 Require Import hvhdl.Place.
 
 Require Import sitpn2hvhdl.Sitpn2HVhdl.
+Require Import sitpn2hvhdl.Sitpn2HVhdlInvs.
 Require Import sitpn2hvhdl.GenerateInfosFacts.
 Require Import sitpn2hvhdl.GenerateArchitectureFacts.
-Require Import sitpn2hvhdl.GeneratePortsFacts.
 
 (** ** Facts about [InputMap_to_AST] Function *)
 
 Section InputMap2AST.
-
-  Lemma imap_entry_to_associp_inv_state :
-    forall {sitpn im ime s v s'},
-      imap_entry_to_associp sitpn im ime s = OK v s' ->
-      s = s'.
-  Proof.
-    unfold imap_entry_to_associp.
-    destruct ime; destruct s; intros s v s' e1; monadFullInv e1;
-      [ auto | destruct l; monadFullInv EQ; auto ].
-  Qed.
-
-  Lemma InputMap_to_AST_inv_state :
-    forall {sitpn imap s ipm s'},
-      InputMap_to_AST sitpn imap s = OK ipm s' ->
-      s = s'.
-  Proof.
-    unfold InputMap_to_AST; intros.
-    eapply foldl_inv_state; eauto with typeclass_instances;
-      intros; eapply imap_entry_to_associp_inv_state; eauto.
-  Qed.
 
   Lemma foldl_imap_entry_to_associp_In_inl :
     forall {sitpn imap s ipm1 ipm2 s' id e},
@@ -87,43 +57,12 @@ End InputMap2AST.
 (** ** Facts about [OutputMap_to_AST] Function *)
 
 Section OutputMap2AST.
-
-  Lemma omap_entry_to_assocop_inv_state :
-    forall {sitpn om ome s v s'},
-      omap_entry_to_assocop sitpn om ome s = OK v s' ->
-      s = s'.
-  Proof.
-    unfold omap_entry_to_assocop.
-    destruct ome; destruct s; intros s v s' e1; monadFullInv e1;
-      [ auto | destruct l; monadFullInv EQ; auto ].
-  Qed.
-
-  Lemma OutputMap_to_AST_inv_state :
-    forall {sitpn omap s opm s'},
-      OutputMap_to_AST sitpn omap s = OK opm s' ->
-      s = s'.
-  Proof.
-    unfold OutputMap_to_AST; intros.
-    eapply foldl_inv_state; eauto with typeclass_instances;
-      intros; eapply omap_entry_to_assocop_inv_state; eauto.
-  Qed.
   
 End OutputMap2AST.
 
 (** ** Facts about [HComponent_to_comp_inst] Function *)
 
 Section HComp2CompInst.
-
-  Lemma HComp_to_comp_inst_inv_state :
-    forall {sitpn id__c id__e hcomp s v s'},
-      HComponent_to_comp_inst sitpn id__c id__e hcomp s = OK v s' ->
-      s = s'.
-  Proof.
-    intros until s'; intros e; destruct hcomp as ((gm, ipm), opm).
-    monadFullInv e; transitivity s0.
-    eapply InputMap_to_AST_inv_state; eauto.
-    eapply OutputMap_to_AST_inv_state; eauto.
-  Qed.
 
   Lemma HComp_to_comp_inst_p_comp :
     forall {sitpn id__c id__e hcomp s v s'},
@@ -143,55 +82,7 @@ End HComp2CompInst.
 Section GeneratePlaceCompInst.
 
   (** *** P Component Generation *)
-  
-  Lemma gen_pcomp_inst_inv_p_comp_1 :
-    forall {sitpn x y s v s' id__p gm ipm opm},
-      generate_place_comp_inst sitpn y s = OK v s' ->
-      ~Peq x y ->
-      InA Pkeq (x, id__p) (p2pcomp (γ s)) ->
-      InCs (cs_comp id__p Petri.place_entid gm ipm opm) (beh s) ->
-      InA Pkeq (x, id__p) (p2pcomp (γ s')) /\
-      InCs (cs_comp id__p Petri.place_entid gm ipm opm) (beh s').
-  Proof.
-    intros until opm; intros e; intros; split;
-      monadFullInv e; simpl; simpl in EQ4;
-        specialize (getv_inv_state EQ4) as e1;
-        specialize (HComp_to_comp_inst_inv_state EQ2) as e2;
-        rewrite <- e2, <- e1; clear e1 e2; simpl;
-          [ apply InA_setv_inv_1; auto | right; assumption ].
-  Qed.
-
-  Lemma gen_pcomp_inst_inv_p_comp_2 :
-    forall {sitpn x y s v s' id__p gm ipm opm},
-      generate_place_comp_inst sitpn y s = OK v s' ->
-      ~Peq x y ->
-      InA Pkeq (x, id__p) (p2pcomp (γ s')) ->
-      InCs (cs_comp id__p Petri.place_entid gm ipm opm) (beh s') ->
-      ~(exists p1 id__p1, InA Pkeq (p1, id__p1) (p2pcomp (γ s)) /\ id__p1 >= nextid s) ->
-      InA Pkeq (x, id__p) (p2pcomp (γ s)) /\
-      InCs (cs_comp id__p Petri.place_entid gm ipm opm) (beh s).
-  Proof.
-    intros until opm; intros e nPeq InA_p2pcomp InCs_beh; minv e; shelf_state EQ5.
-    (* Stores the first subgoal (need it in the second subgoal). *)
-    assert (InA_p2pcomp0 : InA Pkeq (x, id__p) (p2pcomp (γ s0))).
-    { eapply @InA_setv_inv_2 with (eqk_dec := Peqdec) (v := nextid s0); eauto.
-      change (setv Peqdec y (nextid s0) (p2pcomp (γ s0))) with (p2pcomp (γ s)).
-      assert (e : p2pcomp (γ s4) = (p2pcomp (γ s))).
-      { rewrite (getv_inv_state EQ5), (InputMap_to_AST_inv_state EQ3),
-        (OutputMap_to_AST_inv_state EQ2); reflexivity. }
-      rewrite <- e; auto. }
-    intros nex_InA; split; auto.
-    (* SUBGOAL [comp(id__p, "place", ...) ∈ (beh s0)] *)
-    destruct InCs_beh as [eq_comp | InCs_beh4].
-    (* CASE comp. are equal. *)
-    inject_left eq_comp; exfalso; apply nex_InA; exists x, (nextid s0); auto.
-    (* CASE [comp ∈ beh s0] *)
-    assert (e : beh s = beh s4).
-    { rewrite (getv_inv_state EQ5), (InputMap_to_AST_inv_state EQ3),
-      (OutputMap_to_AST_inv_state EQ2); reflexivity. }
-    change (beh s0) with (beh s); rewrite e; auto.
-  Qed.
-  
+    
   Lemma gen_p_comp_inst_p_comp :
     forall {sitpn p s v s'},
       generate_place_comp_inst sitpn p s = OK v s' ->
@@ -258,140 +149,8 @@ Section GeneratePlaceCompInst.
       [ apply (proj2 SIL) | apply ((proj1 SIL) p)].
   Qed.
 
-  (** *** NoDup in p2pcomp *)
-  
-  Lemma gen_p_comp_inst_nodup_p2pcomp :
-    forall {sitpn p s v s'},
-      generate_place_comp_inst sitpn p s = OK v s' ->
-      ~InA Peq p (fs (p2pcomp (γ s))) ->
-      NoDupA Peq (fs (p2pcomp (γ s))) ->
-      NoDupA Peq (fs (p2pcomp (γ s'))).
-  Proof.
-    intros until s'; intros e; monadFullInv e;
-      simpl; simpl in EQ4;
-        specialize (getv_inv_state EQ4) as e1;
-        specialize (HComp_to_comp_inst_inv_state EQ2) as e2;
-        rewrite <- e2, <- e1; clear e1 e2; simpl.
-    do 1 intro; apply NoDupA_setv_cons; auto.
-  Qed.
-
-  Lemma gen_p_comp_inst_inv_p2pcomp :
-    forall {sitpn x y s v s'},
-      generate_place_comp_inst sitpn y s = OK v s' ->
-      ~Peq y x ->
-      ~InA Peq x (fs (p2pcomp (γ s))) ->
-      ~InA Peq x (fs (p2pcomp (γ s'))).
-  Proof.
-    intros until s'; intros e; intros;
-      monadFullInv e; simpl; simpl in EQ4;
-        specialize (getv_inv_state EQ4) as e1;
-        specialize (HComp_to_comp_inst_inv_state EQ2) as e2;
-        rewrite <- e2, <- e1; clear e1 e2; simpl; auto with setoidl.
-  Qed.
-
-  Lemma iter_gen_pcomp_inst_inv_nodup_p2pcomp :
-    forall {sitpn pls} {s v s'},
-      iter (generate_place_comp_inst sitpn) pls s = OK v s' ->
-      forall p,
-        ~InA Peq p (fs (p2pcomp (γ s))) ->
-        ~InA Peq p pls ->
-        ~InA Peq p (fs (p2pcomp (γ s'))).
-  Proof.
-    intros until pls;
-      functional induction (iter (generate_place_comp_inst sitpn) pls) using iter_ind;
-      intros s v s' e; monadInv e; auto; intros.
-    eapply gen_p_comp_inst_inv_p2pcomp; eauto with setoidl.
-    intro; apply H0; symmetry in H1; auto.
-  Qed.
-
-  Lemma iter_gen_pcomp_inst_nodup_p2pcomp :
-    forall {sitpn pls s v s'},
-      iter (generate_place_comp_inst sitpn) pls s = OK v s' ->
-      NoDupA Peq pls ->
-      (forall p, InA Peq p pls -> ~InA Peq p (fs (p2pcomp (γ s)))) ->
-      NoDupA Peq (fs (p2pcomp (γ s))) ->
-      NoDupA Peq (fs (p2pcomp (γ s'))).
-  Proof.
-    intros until pls;
-      functional induction (iter (generate_place_comp_inst sitpn) pls) using iter_ind;
-      intros s v s' e; monadInv e; auto; intros.
-    
-    eapply gen_p_comp_inst_nodup_p2pcomp; eauto;
-      lazymatch goal with
-      | [ Hnd: NoDupA _ (?a :: ?tl), Hnin: forall _, _ -> ~_ |- _ ] =>
-        (eapply iter_gen_pcomp_inst_inv_nodup_p2pcomp; eauto; [
-           apply Hnin; apply InA_cons_hd; reflexivity
-         | inversion Hnd; assumption])
-        || (eapply IHm; eauto; inversion Hnd; assumption)
-      end.
-  Qed.
-
   (** *** Bind initial marking *)
-
-  Lemma gen_p_comp_inst_inv_nextid_2 :
-    forall {sitpn p s v s'},
-      generate_place_comp_inst sitpn p s = OK v s' ->
-      ~(exists p id__p, InA Pkeq (p, id__p) (p2pcomp (γ s)) /\ id__p >= nextid s) ->
-      ~(exists p id__p, InA Pkeq (p, id__p) (p2pcomp (γ s')) /\ id__p >= nextid s').
-  Proof.
-    intros until s'; intros e; minv e; shelf_state EQ5.
-    intros nex_InA; destruct 1 as (p1, (id__p1, (InA_p2pcomp0, GE_nxtid0))).
-    assert (s = s2) by (eapply getv_inv_state; eauto); subst.
-    assert (s = s3) by (eapply InputMap_to_AST_inv_state; eauto); subst.
-    assert (s = s4) by (eapply OutputMap_to_AST_inv_state; eauto); subst.
-    change (p2pcomp (γ s))
-      with (setv Peqdec p (nextid s0) (p2pcomp (γ s0))) in InA_p2pcomp0.
-    edestruct @InA_setv_fst_or_in_tl as [(Peq_, e) | InA_beh0]; eauto.
-    (* CASE [Peq p1 p] and [id__p1 = nextid s0] *)
-    subst; change (nextid s) with (S (nextid s0)) in GE_nxtid0; lia.
-    (* CASE [InA Pkeq (p1, id__p1) (p2pcomp (γ s0))] *)
-    apply nex_InA; exists p1, id__p1; split;
-      [ assumption | change (nextid s) with (S (nextid s0)) in GE_nxtid0; lia ].
-  Qed.
-
-  Lemma iter_gen_pcomp_inst_inv_nextid_2 :
-    forall {sitpn pls} {s v s'},
-      iter (generate_place_comp_inst sitpn) pls s = OK v s' ->
-      ~(exists p id__p, InA Pkeq (p, id__p) (p2pcomp (γ s)) /\ id__p >= nextid s) ->
-      ~(exists p id__p, InA Pkeq (p, id__p) (p2pcomp (γ s')) /\ id__p >= nextid s').
-  Proof.
-    intros until s'; intros e; solve_listm e.
-    intros; eapply gen_p_comp_inst_inv_nextid_2; eauto.
-  Qed.
-  
-  Lemma gen_p_comp_inst_inv_nextid_1 :
-    forall {sitpn p s v s'},
-      generate_place_comp_inst sitpn p s = OK v s' ->
-      ~(exists id__c id__e g i o, InCs (cs_comp id__c id__e g i o) (beh s) /\ id__c >= nextid s) ->
-      ~(exists id__c id__e g i o, InCs (cs_comp id__c id__e g i o) (beh s') /\ id__c >= nextid s').
-  Proof.
-    intros until s'; intros e; minv e; shelf_state EQ5.
-    intros nex_InCs; destruct 1 as (id__c, (id__e, (g1, (i1, (o1, (InCs_or, GE_nxtid)))))).
-    destruct InCs_or as [eq_comp | InCs_beh ].
-    (* CASE comp. are equal *)
-    inject_left eq_comp.
-    assert (s = s2) by (eapply getv_inv_state; eauto); subst.
-    assert (s = s3) by (eapply InputMap_to_AST_inv_state; eauto); subst.
-    assert (s = s4) by (eapply OutputMap_to_AST_inv_state; eauto); subst.
-    change (nextid s) with (S (nextid s0)) in GE_nxtid; lia.
-    (* CASE [comp(id__c, id__e, g1, i1, o1) ∈ (beh s4)] *)
-    apply nex_InCs; exists id__c, id__e, g1, i1, o1.
-    assert (s = s2) by (eapply getv_inv_state; eauto); subst.
-    assert (s = s3) by (eapply InputMap_to_AST_inv_state; eauto); subst.
-    assert (s = s4) by (eapply OutputMap_to_AST_inv_state; eauto); subst.
-    split; auto; cbn in GE_nxtid; lia.
-  Qed.
     
-  Lemma iter_gen_pcomp_inst_inv_nextid_1 :
-    forall {sitpn pls} {s v s'},
-      iter (generate_place_comp_inst sitpn) pls s = OK v s' ->
-      ~(exists id__c id__e g i o, InCs (cs_comp id__c id__e g i o) (beh s) /\ id__c >= nextid s) ->
-      ~(exists id__c id__e g i o, InCs (cs_comp id__c id__e g i o) (beh s') /\ id__c >= nextid s').
-  Proof.
-    intros until s'; intros e; solve_listm e.
-    intros; eapply gen_p_comp_inst_inv_nextid_1; eauto.
-  Qed.
-  
   Lemma gen_pcomp_inst_bind_init_marking :
     forall {sitpn p s v s' g i o},
       generate_place_comp_inst sitpn p s = OK v s' ->
@@ -425,19 +184,6 @@ Section GeneratePlaceCompInst.
       erewrite @eqv_if_InA_NoDupA_setv with (y := id__p) (eqk := Peq) in InCs_beh;
       eauto with typeclass_instances.
     exfalso; apply nex_InCs; exists Petri.place_entid, gm, ipm, opm; auto.
-  Qed.
-
-  Lemma iter_gen_pcomp_inst_inv_arch :
-    forall {sitpn pls} {s v s'},
-      iter (generate_place_comp_inst sitpn) pls s = OK v s' ->
-      arch s = arch s'.
-  Proof. intros *; intros e; solve_listm e.
-         intros *; intros e; minv e.
-         shelf_state EQ5; change (arch s0) with (arch s1).
-         rewrite (getv_inv_state EQ5),
-         (InputMap_to_AST_inv_state EQ3),
-         (OutputMap_to_AST_inv_state EQ2).
-         reflexivity.
   Qed.
   
   Lemma iter_gen_pcomp_inst_bind_init_marking :
@@ -516,102 +262,7 @@ End GeneratePlaceCompInst.
 (** ** Facts about Generation of T Component Instances *)
 
 Section GenerateTransCompInst.
-
-  Lemma gen_t_comp_inst_inv_p2pcomp :
-    forall {sitpn t s v s'},
-      generate_trans_comp_inst sitpn t s = OK v s' ->
-      p2pcomp (γ s) = p2pcomp (γ s').
-  Proof.
-    intros until s'; intros e; monadFullInv e; simpl; simpl in EQ3.
-    specialize (getv_inv_state EQ3) as e1;
-      specialize (HComp_to_comp_inst_inv_state EQ0) as e2;
-      rewrite <- e2, <- e1; clear e1 e2; simpl; reflexivity.
-  Qed.
-  
-  Lemma iter_gen_tcomp_inst_inv_p2pcomp :
-    forall {sitpn trs s v s'},
-      iter (generate_trans_comp_inst sitpn) trs s = OK v s' ->
-      p2pcomp (γ s) = p2pcomp (γ s').
-  Proof.
-    intros until s'; intros e; solveSInv e.
-    intros; eapply gen_t_comp_inst_inv_p2pcomp; eauto.
-  Qed.
-  
-  Lemma gen_t_comp_inst_inv_in_beh :
-    forall {sitpn t s v s'},
-      generate_trans_comp_inst sitpn t s = OK v s' ->
-      forall cstmt,
-        InCs cstmt (beh s) -> InCs cstmt (beh s').
-  Proof.
-    intros until s'; intros e; monadFullInv e; simpl; simpl in EQ3.
-    specialize (getv_inv_state EQ3) as e1;
-      specialize (HComp_to_comp_inst_inv_state EQ0) as e2;
-      rewrite <- e2, <- e1; clear e1 e2; simpl.
-    intros; right; assumption.
-  Qed.
-
-  Lemma iter_gen_tcomp_inst_inv_in_beh :
-    forall {sitpn trs s v s'},
-      iter (generate_trans_comp_inst sitpn) trs s = OK v s' ->
-      forall cstmt, InCs cstmt (beh s) -> InCs cstmt (beh s').
-  Proof.
-    intros until s'; intros e; solveSInv e.
-    intros; eapply gen_t_comp_inst_inv_in_beh; eauto.
-  Qed.
-  
-  Lemma gen_tcomp_insts_inv_p_comp :
-    forall {sitpn s v s' p id__p gm ipm opm},
-      generate_trans_comp_insts sitpn s = OK v s' ->
-      InA Pkeq (p, id__p) (p2pcomp (γ s)) ->
-      InCs (cs_comp id__p Petri.place_entid gm ipm opm) (beh s) ->
-      InA Pkeq (p, id__p) (p2pcomp (γ s')) /\
-      InCs (cs_comp id__p Petri.place_entid gm ipm opm) (beh s').
-  Proof.
-    intros until opm; intros e; monadFullInv e.
-    split;
-      [rewrite <- (iter_gen_tcomp_inst_inv_p2pcomp EQ0); assumption |
-       eapply iter_gen_tcomp_inst_inv_in_beh; eauto].
-  Qed.
-
-  Lemma gen_tcomp_insts_inv_p2pcomp :
-    forall {sitpn s v s'},
-      generate_trans_comp_insts sitpn s = OK v s' ->
-      p2pcomp (γ s) = p2pcomp (γ s').
-  Proof.
-    intros *; intros e; minv e.
-    eapply iter_gen_tcomp_inst_inv_p2pcomp; eauto.
-  Qed.
-
-  Lemma gen_tcomp_inst_gen_only_tcomp :
-    forall {sitpn t s v s'},
-      generate_trans_comp_inst sitpn t s = OK v s' ->
-      forall {id__c id__e gm ipm opm},
-        id__e <> Petri.transition_entid ->
-        InCs (cs_comp id__c id__e gm ipm opm) (beh s') ->
-        InCs (cs_comp id__c id__e gm ipm opm) (beh s).
-  Proof.
-    intros *; intros e; minv e; shelf_state EQ4.
-    inversion_clear 2 as [eq_comp | InCs_beh5 ];
-      [ inject_left eq_comp; contradiction | ].
-    change (beh s0) with (beh s).
-    rewrite (getv_inv_state EQ4),
-    (InputMap_to_AST_inv_state EQ2),
-    (OutputMap_to_AST_inv_state EQ0); auto.
-  Qed.
-  
-  Lemma gen_tcomp_insts_gen_only_tcomp :
-    forall {sitpn s v s'},
-      generate_trans_comp_insts sitpn s = OK v s' ->
-      forall {id__c id__e gm ipm opm},
-        id__e <> Petri.transition_entid ->
-        InCs (cs_comp id__c id__e gm ipm opm) (beh s') ->
-        InCs (cs_comp id__c id__e gm ipm opm) (beh s).
-  Proof.
-    intros *; intros e; minv e.
-    pattern s0, s'; solve_listm EQ0.
-    intros *; eapply gen_tcomp_inst_gen_only_tcomp; eauto.
-  Qed.
-  
+      
 End GenerateTransCompInst.
 
 (** ** Facts about SITPN-to-H-VHDL Transformation Function *)
@@ -775,7 +426,7 @@ Section Sitpn2HVhdl.
     exact (nodup_pls (wi_fsets IWD_sitpn)).
 
     (* SUBGOAL [NoDupA Peq (fs (plmap (arch s1)))] *)
-    eapply gen_ports_sil_plmap; eauto.
+    eapply gen_ports_inv_sil_plmap; eauto.
     eapply gen_arch_sil_plmap; eauto.
     eapply gen_sitpn_infos_sil_lofPs; eauto.
     exact (nodup_pls (wi_fsets IWD_sitpn)).
