sitpn2hvhdl/GenerateInfosFacts.v
@@ -1,6 +1,7 @@
 (** * Facts about Sitpn Information Generation Functions *)
 
 Require Import common.Coqlib.
+Require Import common.GlobalFacts.
 Require Import common.StateAndErrorMonad.
 Require Import common.StateAndErrorMonadTactics.
 Require Import common.ListDep.
@@ -8,100 +9,22 @@ Require Import common.ListMonad.
 Require Import common.ListMonadFacts.
 Require Import common.ListMonadTactics.
 Require Import common.ListPlus.
-Require Import common.GlobalFacts.
-
 
 Require Import sitpn.dp.Sitpn.
 Require Import sitpn.dp.SitpnFacts.
 
 Require Import sitpn2hvhdl.Sitpn2HVhdl.
+Require Import sitpn2hvhdl.GenerateInfosInvs.
 
 (** ** Facts about Transition Information Generation *)
 
 Section TInfos.
-
-  Lemma gen_tinfos_inv_γ :
-    forall {sitpn s v s'},
-      generate_trans_infos sitpn s = OK v s' ->
-      γ s = γ s'.
-  Proof.
-    intros until s'; intros e; solveSInv e. 
-    intros until s2; intros e1; pattern s1, s2; minv e1; simpl; reflexivity.
-  Qed.
-
-  Lemma gen_tinfos_inv_lofPs :
-    forall {sitpn s v s'},
-      generate_trans_infos sitpn s = OK v s' ->
-      lofPs s = lofPs s'.
-  Proof.
-    intros until s'; intros e; solveSInv e. 
-    intros until s2; intros e1; pattern s1, s2; minv e1; simpl; reflexivity.
-  Qed.
-    
+  
 End TInfos.
 
 (** ** Facts about Place Information Generation *)
 
 Section PInfos.
-
-  Lemma all_conflicts_solved_by_mutex_inv_state :
-    forall {sitpn lofTs s v s'},
-      all_conflicts_solved_by_mutex sitpn lofTs s = OK v s' ->
-      s = s'.
-  Proof.
-    induction lofTs; simpl; intros until s'; intros e; minv e; auto; transitivity s0.
-    - solve_listm EQ1;
-        intros *; intros e; unfold not_exists_mutex in e; minv e;
-          repeat (match goal with
-                  | [e: _ ?st = OK _ _ |- ?st = _ ] => solve_listm e
-                  end).
-    - minv EQ0; auto.
-    - solve_listm EQ1;
-        intros *; intros e; unfold not_exists_mutex in e; minv e;
-          repeat (match goal with
-                  | [e: _ ?st = OK _ _ |- ?st = _ ] => solve_listm e
-                  end).
-    - eapply IHlofTs; eauto.
-  Qed.
-
-  Lemma sort_by_priority_inv_state :
-    forall {sitpn decpr lofTs s v s'},
-      sort_by_priority sitpn decpr lofTs s = OK v s' ->
-      s = s'.
-  Proof.
-    intros until s'; intros e; unfold sort_by_priority in e.
-    eapply foldl_inv_state; eauto with typeclass_instances.
-    intros until s0; cbv beta.
-    functional induction (inject_t sitpn decpr a b) using inject_t_ind;
-      intros until s0'; intros f; minv f; auto.
-    eapply IHc; eauto. 
-  Qed.
-
-  Lemma gen_pinfos_inv_γ :
-    forall {sitpn decpr s v s'},
-      generate_place_infos sitpn decpr s = OK v s' ->
-      γ s = γ s'.
-  Proof.
-    intros until s'; intros e; solveSInv e.
-    intros until s2; intros e1; pattern s1, s2; monadInv e1; simpl.
-    transitivity (γ s).
-    minv EQ; auto.
-    minv EQ1; ((rewrite (all_conflicts_solved_by_mutex_inv_state EQ2); simpl; reflexivity)
-               || (rewrite (all_conflicts_solved_by_mutex_inv_state EQ2), (sort_by_priority_inv_state EQ1); simpl; reflexivity)).
-  Qed.
-
-  Lemma gen_pinfos_inv_lofPs :
-    forall {sitpn decpr s v s'},
-      generate_place_infos sitpn decpr s = OK v s' ->
-      lofPs s = lofPs s'.
-  Proof.
-    intros until s'; intros e; solveSInv e.
-    intros until s2; intros e1; pattern s1, s2; monadInv e1; simpl.
-    transitivity (lofPs s).
-    minv EQ; auto.
-    minv EQ1; ((rewrite (all_conflicts_solved_by_mutex_inv_state EQ2); simpl; reflexivity)
-               || (rewrite (all_conflicts_solved_by_mutex_inv_state EQ2), (sort_by_priority_inv_state EQ1); simpl; reflexivity)).
-  Qed.
   
 End PInfos.
 
@@ -109,77 +32,12 @@ End PInfos.
 
 Section InterprInfos.
 
-  Lemma gen_cinfos_inv_γ :
-    forall {sitpn s v s'},
-      generate_cond_infos sitpn s = OK v s' ->
-      γ s = γ s'.
-  Proof.
-    intros until s'; intros e; pattern s, s'; solveSInv e.
-    intros until s2; intros e1; pattern s1, s2; minv e1; simpl; reflexivity.
-  Qed.
-
-  Lemma gen_cinfos_inv_lofPs :
-    forall {sitpn s v s'},
-      generate_cond_infos sitpn s = OK v s' ->
-      lofPs s = lofPs s'.
-  Proof.
-    intros until s'; intros e; pattern s, s'; solveSInv e.
-    intros until s2; intros e1; pattern s1, s2; minv e1; simpl; reflexivity.
-  Qed.
-  
-  Lemma gen_ainfos_inv_γ :
-    forall {sitpn s v s'},
-      generate_action_infos sitpn s = OK v s' ->
-      γ s = γ s'.
-  Proof.
-    intros until s'; intros e; pattern s, s'; solveSInv e.
-    intros until s2; intros e1; pattern s1, s2; minv e1; simpl; reflexivity.
-  Qed.
-
-  Lemma gen_ainfos_inv_lofPs :
-    forall {sitpn s v s'},
-      generate_action_infos sitpn s = OK v s' ->
-      lofPs s = lofPs s'.
-  Proof.
-    intros until s'; intros e; pattern s, s'; solveSInv e.
-    intros until s2; intros e1; pattern s1, s2; minv e1; simpl; reflexivity.
-  Qed.
-  
-  Lemma gen_finfos_inv_γ :
-    forall {sitpn s v s'},
-      generate_fun_infos sitpn s = OK v s' ->
-      γ s = γ s'.
-  Proof.
-    intros until s'; intros e; pattern s, s'; solveSInv e.
-    intros until s2; intros e1; pattern s1, s2; minv e1; simpl; reflexivity.
-  Qed.
-
-  Lemma gen_finfos_inv_lofPs :
-    forall {sitpn s v s'},
-      generate_fun_infos sitpn s = OK v s' ->
-      lofPs s = lofPs s'.
-  Proof.
-    intros until s'; intros e; pattern s, s'; solveSInv e.
-    intros until s2; intros e1; pattern s1, s2; minv e1; simpl; reflexivity.
-  Qed.
-
 End InterprInfos.
 
 (** ** Facts about Checking of Sitpn Well-definition *)
 
 Section CheckWDSitpn.
 
-  Lemma check_wd_sitpn_inv_eq_state :
-    forall {sitpn decpr s v s'},
-      check_wd_sitpn sitpn decpr s = OK v s' ->
-      s = s'.
-  Proof.  
-    intros until s'; intros e; solveSInv e; auto.
-    intros until s3; intros e1; minv e1; auto.
-    intros until s3; intros e1; solveSInv e1; auto.
-    intros until s5; intros e2; solveSInv e2; auto.
-    intros until s7; intros e3; solveSInv e3; auto.
-  Qed.
   
 End CheckWDSitpn.
 
@@ -226,24 +84,6 @@ Qed.
 
 (** ** Facts about Sitpn Information Generation Function *)
 
-Lemma gen_sitpn_infos_inv_γ :
-  forall {sitpn decpr s v s'},
-    generate_sitpn_infos sitpn decpr s = OK v s' ->
-    γ s = γ s'.
-Proof.
-  intros until s'; intros e; monadInv e.
-  do 10 (match goal with
-        | [ H: ?F _ ?st0 = OK _ ?st1 |- γ ?st0 = γ ?st2 ] =>
-          transitivity (γ st1); [
-            (let e := fresh "e" in solveSInv H; intros *; intros e; minv e; auto)
-            || (minv H; simpl; auto) |];
-          clear H
-        end).
-  rewrite (check_wd_sitpn_inv_eq_state EQ9), (gen_tinfos_inv_γ EQ10), (gen_pinfos_inv_γ EQ11),
-  (gen_cinfos_inv_γ EQ12), (gen_ainfos_inv_γ EQ13).
-  apply (gen_finfos_inv_γ EQ15).
-Qed.
-
 Lemma gen_sitpn_infos_sil_lofPs :
   forall {sitpn decpr s v s'},
     generate_sitpn_infos sitpn decpr s = OK v s' ->
@@ -264,16 +104,4 @@ Proof.
   eapply tmap_aux_sil_lofPs; eauto;
     [intros; left; exact (proj2_sig p) | inversion 1].
 Qed.
-
-Lemma gen_sitpn_infos_inv_arch :
-  forall {sitpn decpr s v s'},
-    generate_sitpn_infos sitpn decpr s = OK v s' ->
-    arch s = arch s'.
-Admitted.
-
-Lemma gen_sitpn_infos_inv_beh :
-  forall {sitpn decpr s v s'},
-    generate_sitpn_infos sitpn decpr s = OK v s' ->
-    beh s = beh s'.
-Admitted.
 
