sitpn2hvhdl/Sitpn2HVhdlFacts.v
@@ -1,0 +1,4 @@
+Require Export sitpn2hvhdl.GenerateInfosFacts.
+Require Export sitpn2hvhdl.GenerateArchitectureFacts.
+Require Export sitpn2hvhdl.GeneratePortsFacts.
+Require Export sitpn2hvhdl.GenerateHVhdlFacts.
